\documentclass[12pt]{article}
\usepackage{amsmath, amssymb}
\usepackage{enumitem}
\usepackage[margin=1in]{geometry}

\begin{document}

\title{SAT Math Practice Questions: Solutions}
\author{Generated by Grok 3 (xAI)}
\date{April 07, 2025}
\maketitle
\tableofcontents
\newpage

\section{Algebra Solutions}
\begin{enumerate}[label=\textbf{Question \arabic*:}]
  \item \( 2x + 3 = 11 \Rightarrow x = 4 \) \textbf{(B)}
  \item \( 3(x - 2) = 2x + 5 \Rightarrow x = 11 \) \textbf{(C)}
  \item \( 2x - 7 = 3 \Rightarrow x = 5 \Rightarrow 4x + 5 = 25 \) \textbf{(B)}
  \item \( x + y = 7, 2x - y = 3 \Rightarrow x = \frac{10}{3}, y = \frac{11}{3} \) \textbf{(D)}
  \item \( f(x) = 3x + 2 \Rightarrow f(4) = 14 \) \textbf{(B)}
  \item \( x^2 - 5x + 6 = (x - 2)(x - 3) \) \textbf{(B)}
  \item \( x^2 - 4x - 5 = 0 \Rightarrow x = 5, -1 \) \textbf{(B)}
  \item \( \frac{3}{x} = 6 \Rightarrow x = \frac{1}{2} \) \textbf{(A)}
  \item \( \frac{2x}{3} - \frac{1}{2} = \frac{3}{4} \Rightarrow x = \frac{15}{8} \)
  \item \( \frac{2}{3}x - \frac{1}{4}(6x - 8) = -\frac{5x}{6} + 2 \)
  \item \( 2(3x - 4) - 5(x - 1) = x - 3 \) \textbf{(A)}
  \item \( x^2 - 4x + 3 = 0 \Rightarrow x = 1, 3 \) \textbf{(A)}
  \item \( (x + 2)^2 = x^2 + 4x + 4 \) \textbf{(B)}
  \item \( \frac{x}{2} + \frac{x}{3} = 5 \Rightarrow x = 6 \)
  \item \( 4x^2 - 12x + 9 = (2x - 3)^2 \)
  \item \( \frac{x^2 - 9}{x - 3} = x + 3 \) \textbf{(A)}
  \item \( |2x - 5| = 3 \Rightarrow x = 4, 1 \) \textbf{(A)}
  \item \( 6x^2 + 11x - 10 = (2x + 5)(3x - 2) \) \textbf{(B)}
  \item \( \frac{2}{x - 1} = \frac{4}{x + 1} \Rightarrow x = 3 \)
  \item Roots 2, -3: \( x^2 + x - 6 \)
  \item \( 2(x - 3) = 4x + 2 \Rightarrow x = -4 \) \textbf{(C)}
  \item \( |3x + 1| = 7 \Rightarrow x = 2, -\frac{8}{3} \) \textbf{(A)}
  \item \( 6x^2 + 11x - 35 = (2x + 7)(3x - 5) \) \textbf{(A)}
  \item \( \frac{2x}{x - 3} = 4 \Rightarrow x = 6 \) \textbf{(C)}
  \item \( x + 2y = 7, 2x - y = 1 \Rightarrow x = \frac{9}{5}, y = \frac{13}{5} \) \textbf{(A)}
  \item \( (x + 3)(2x - 4) = 2x^2 + 2x - 12 \) \textbf{(A)}
  \item \( x^2 + 5x + 6 = 0 \Rightarrow x = -2, -3 \) \textbf{(A)}
  \item \( \frac{3x}{4} - \frac{2x}{3} = \frac{x}{12} \) \textbf{(A)}
  \item \( \frac{1}{x} + \frac{1}{x + 2} = \frac{3}{4} \Rightarrow x = -\frac{4}{3}, 2 \)
  \item \( x^3 - 27 = (x - 3)(x^2 + 3x + 9) \)
\end{enumerate}

\newpage

\section{Geometry and Trigonometry Solutions}
\begin{enumerate}[label=\textbf{Question \arabic*:}]
  \item \( 3 \times 4 = 12 \) \textbf{(B)}
  \item Hypotenuse = \( 2 \times 5 = 10 \) \textbf{(B)}
  \item \( 2\pi r = 10\pi \Rightarrow r = 5 \Rightarrow A = 25\pi \) \textbf{(A)}
  \item \( x^2 + y^2 = 25 \Rightarrow \frac{dy}{dx} = -\frac{3}{4} \) at (3,4)
  \item \( 180^\circ - 45^\circ - 60^\circ = 75^\circ \)
  \item \( \pi r^2 = 49\pi \Rightarrow r = 7 \) \textbf{(B)}
  \item \( \sin 30^\circ = \frac{\text{opp}}{10} \Rightarrow \text{opp} = 5 \) \textbf{(A)}
  \item Perimeter = \( 2(3 + 3) = 12 \) \textbf{(B)}
  \item \( 3k + 4k + 5k = 180^\circ \Rightarrow 5k = 75^\circ \) \textbf{(B)}
  \item \( \sin \theta = \frac{1}{2} \Rightarrow \theta = 30^\circ \) \textbf{(A)}
  \item \( (x - 2)^2 + (y + 3)^2 = 16 \) \textbf{(A)}
  \item \( 5 = 2\theta \Rightarrow \theta = 2.5 \) \textbf{(A)}
  \item \( \frac{1}{2} \cdot 8 \cdot 5 = 20 \) \textbf{(A)}
  \item Midpoint = \( (1, 2) \)
  \item \( \cos x = \frac{\sqrt{2}}{2} \Rightarrow x = 45^\circ, 315^\circ \)
  \item \( 2\pi r = 18\pi \Rightarrow r = 9 \) \textbf{(A)}
  \item \( \sqrt{3^2 + 4^2} = 5 \) \textbf{(A)}
  \item Heronâ€™s: \( s = 12, A \approx 27 \) \textbf{(B)}
  \item Slope = 2, \( y = 2x - 1 \)
  \item \( \tan x = 1 \Rightarrow x = 45^\circ, 225^\circ \)
  \item \( 3 \times 4 = 12 \) \textbf{(B)}
  \item Hypotenuse = \( 2 \times 5 = 10 \) \textbf{(B)}
  \item \( 2\pi r = 10\pi \Rightarrow A = 25\pi \) \textbf{(A)}
  \item Slope = \( -\frac{3}{4} \) (same as Q4)
  \item \( 75^\circ \) (same as Q5)
  \item \( \pi \cdot 7^2 = 49\pi \) \textbf{(A)}
  \item \( \pi \cdot 10 = 10\pi \) \textbf{(A)}
  \item Hypotenuse = \( 2 \cdot 6 = 12 \) \textbf{(C)}
  \item \( \frac{80^\circ}{2} = 40^\circ \) \textbf{(A)}
  \item \( \sin 45^\circ = \frac{\sqrt{2}}{2} \) \textbf{(A)}
  \item \( \cos 60^\circ = \frac{1}{2} \) \textbf{(A)}
  \item \( \sqrt{3^2 + 4^2} = 5 \) \textbf{(A)}
  \item Side = 10 \textbf{(B)}
  \item \( \frac{120^\circ}{2} = 60^\circ \)
  \item \( \cos 37^\circ \approx 0.8 \Rightarrow h = 10 \)
\end{enumerate}

\newpage

\section{Problem Solving and Data Analysis Solutions}
\begin{enumerate}[label=\textbf{Question \arabic*:}]
  \item \( 0.3 \cdot 120 = 36 \) \textbf{(A)}
  \item \( 5 \cdot 12 = 60 \) \textbf{(A)}
  \item \( 0.4 \cdot 200 = 80 \) \textbf{(A)}
  \item \( \frac{2}{3} \cdot 15 = 10 \) \textbf{(C)}
  \item \( \frac{150}{3} = 50 \) mph \textbf{(A)}
  \item \( 1 - \frac{3}{8} = \frac{5}{8} \) \textbf{(A)}
  \item \( 1.2 \cdot 0.8 = 0.96 \Rightarrow 4\% \) decrease \textbf{(B)}
  \item \( 2(2w + w) = 36 \Rightarrow w = 6, A = 72 \) \textbf{(C)}
  \item \( \frac{7}{20} \)
  \item Median = 3
  \item Middle value = 8 \textbf{(B)}
  \item \( \frac{5}{10} = \frac{1}{2} \) \textbf{(A)}
  \item \( y = 2(4) + 1 = 9 \) \textbf{(C)}
  \item Mean = 7.4, SD \(\approx\) 1.62
  \item \( 40 - (18 + 15 - 5) = 12 \)
  \item \( 0.7 \cdot 50 = 35 \) \textbf{(B)}
  \item Mode = 3 \textbf{(B)}
  \item \( \frac{5}{10} = \frac{1}{2} \) \textbf{(A)}
  \item Range = 7, IQR = 5
  \item Weighted average = 81.5
  \item \( 12 \cdot \frac{8}{5} = 19.20 \) \textbf{(A)}
  \item \( \frac{2}{3} \cdot 9 = 6 \) \textbf{(C)}
  \item \( \binom{8}{4} \left(\frac{1}{2}\right)^8 \) \textbf{(A)}
  \item \( 60 \cdot 2.5 = 150 \) \textbf{(C)}
  \item \( 0.75x = 45 \Rightarrow x = 60 \) \textbf{(C)}
  \item \( 300 - 0.6 \cdot 300 = 120 \) \textbf{(C)}
  \item \( 90 - (16 + 20 + 15 + 22) = 17 \) \textbf{(A)}
  \item \( w = 6, l = 12 \Rightarrow A = 72 \) \textbf{(C)}
  \item Median = 6
  \item Range = 100, Mean = 200
\end{enumerate}

\newpage

\section{Advanced Math Solutions}
\begin{enumerate}[label=\textbf{Question \arabic*:}]
  \item \( x^2 - 2x - 8 = 0 \Rightarrow x = 4, -2 \) \textbf{(B)}
  \item \( f(2) = 2(4) - 3(2) + 1 = 3 \) \textbf{(A)}
  \item \( \sqrt{2x + 5} = 3 \Rightarrow x = 2 \) \textbf{(B)}
  \item \( 16^{\frac{3}{4}} = 8 \) \textbf{(C)}
  \item \( \frac{3x^2 - 12}{3} = x^2 - 4 = (x - 2)(x + 2) \) \textbf{(D)}
  \item \( 2x - 5 < 3 \Rightarrow x < 4 \) \textbf{(B)}
  \item Horizontal asymptote: \( y = 0 \) \textbf{(B)}
  \item \( \log_2(32) = 5 \) \textbf{(B)}
  \item \( f^{-1}(x) = \frac{2x + 1}{3} \)
  \item \( \frac{1}{1 + \frac{1}{x}} = \frac{x}{x + 1} \)
  \item \( (x + 3)^2 = 0 \Rightarrow x = -3 \) \textbf{(A)}
  \item \( (2x^3)^2 = 4x^6 \) \textbf{(B)}
  \item Vertex: \( (2, 0) \) \textbf{(A)}
  \item \( f'(x) = 6x - 2 \)
  \item \( e^x = 5 \Rightarrow x = \ln 5 \)
  \item \( (x - 3)^2 = 0 \Rightarrow x = 3 \) \textbf{(A)}
  \item \( (3x^2)^2 = 9x^4 \) \textbf{(A)}
  \item Vertex: \( (2, 0) \) \textbf{(A)}
  \item \( f'(x) = 12x^2 - 4x + 1 \)
  \item \( 2^x = 7 \Rightarrow x = \log_2 7 \)
  \item \( (2x + 1)(x - 3) = 0 \Rightarrow x = -\frac{1}{2}, 3 \) \textbf{(A)}
  \item \( \log_3(81) = 4 \) \textbf{(B)}
  \item \( 16^{\frac{3}{4}} = 8 \) \textbf{(A)}
  \item \( \frac{2}{3x^{-2}} = \frac{2x^2}{3} \) \textbf{(A)}
  \item \( f^{-1}(x) = \frac{5x - 3}{2} \) \textbf{(A)}
  \item \( f'(x) = 9x^2 - 4 \) \textbf{(A)}
  \item \( e^x = 20 \Rightarrow x = \ln 20 \) \textbf{(A)}
  \item \( \frac{1}{\sqrt{50}} = \frac{\sqrt{2}}{5} \) \textbf{(B)}
  \item \( \log_2(x - 1)(x + 3) = 3 \Rightarrow x = 3 \)
  \item \( f''(x) = 12x^2 - 12x \)
\end{enumerate}

\end{document}